stacktree.v
@@ -1,0 +1,72 @@
+Require Import Coq.Lists.List.
+Require Import Program.
+
+Import List.ListNotations.
+
+(** * Stack Tree *)
+
+Inductive stree :=
+| Node : list stree    (**r Trees containing inactive frames *)
+       -> option stree  (**r An active sub-stackframe (if any) *)
+       -> stree.
+
+Definition empty_tree := Node [] None.
+
+(* Fixpoint stree_length t :=  *)
+(*   match t with *)
+(*   | Node l None => 0 *)
+(*   | Node l (Some t') => S (stree_length t') *)
+(*   end. *)
+
+(* Fixpoint stree_depth t := *)
+(*   match t with  *)
+(*   | Node l o => *)
+(*     let d := match o with *)
+(*             | None => 0 *)
+(*             | Some t' => stree_depth t' *)
+(*             end  *)
+(*     in *)
+(*     fold_right (fun t' d' => Nat.max (stree_depth t') d') d l *)
+(*   end. *)
+
+(** Fold left and right functions for stree *)
+(* Fixpoint stree_fold_left {A:Type} (f: A -> stree -> A) (t:stree) (acc:A) := *)
+(*   let acc' := f acc t in *)
+(*   match t with *)
+(*   | Node l None => acc' *)
+(*   | Node l (Some t') => stree_fold_left f t' acc' *)
+(*   end. *)
+
+(* Fixpoint stree_fold_right {A:Type} (f: stree -> A -> A) (acc:A) (t:stree) := *)
+(*   match t with *)
+(*   | Node l None => f t acc *)
+(*   | Node l (Some t') => f t' (stree_fold_right f acc t') *)
+(*   end. *)
+
+
+(** Path *)
+Definition path := list nat.
+
+(** Next tree and path *)
+Fixpoint next_stree (t: stree) : (stree * path) :=
+  match t with 
+  | Node l None => 
+    let idx := length l in    
+    (Node l (Some empty_tree), [idx])
+  | Node l (Some t') =>
+    let (t'', p) := next_stree t' in
+    (Node l (Some t''), (length l) :: p)
+  end.
+
+(** Return from the active node (use well-founded induction) *)
+
+Fixpoint return_stree (t: stree) : option stree :=
+  match t with
+  | Node l None =>
+    None
+  | Node l (Some t) =>
+    match return_stree t with
+    | None => Some (Node (l ++ [t]) None)
+    | Some t' => Some (Node l (Some t'))
+    end
+  end.
